\renewcommand{\theequation}{\theenumi}
\begin{enumerate}[label=\thesection.\arabic*.,ref=\thesection.\theenumi]
\numberwithin{equation}{enumi}
\item Now we know the following values:
\begin{align}
\vec{A} &= \begin{pmatrix}r\\0 \end{pmatrix} \\
\vec{B} &= \begin{pmatrix}-r\\0 \end{pmatrix} \\
\vec{C} &= r\begin{pmatrix}\cos\theta\\\sin\theta \end{pmatrix} \\
\vec{D} &= r\begin{pmatrix}\cos\theta_1\\\sin\theta_1 \end{pmatrix} 
\end{align}
where $\theta$=45\degree, $\theta_1$ = 105\degree and $r$=2 units.

\item Let the $\angle AEB$= $\alpha$. Consider the below equation,
\begin{align}
\brak{\vec{D}-\vec{B}}^T\brak{\vec{C} - \vec{A}} &= BD.AC.\cos\alpha
\label{eq:gen}
\end{align}

\item Now finding BD 
\begin{align}
(BD)^2 &= \brak{\vec{D}-\vec{B}}^T\brak{\vec{D}-\vec{B}} \\
       &= r\brak{\cos\theta_1+1 \hspace{0.2cm} \sin\theta_1} r\begin{pmatrix}
       \cos\theta_1+1 \\ \sin\theta_1
       \end{pmatrix} \\
    &= r^2 \brak{1+ \cos^2\theta_1 + 2\cos\theta_1 + \sin^2\theta_1}
\end{align}
Substituting the values of $\theta_1$ and $r$ , we get
\begin{align}
BD &= 2.435
\label{eq:BD}
\end{align}

\item Finding AC 
\begin{align}
(AC)^2 &= \brak{\vec{C}-\vec{A}}^T\brak{\vec{C}-\vec{A}} \\
&= r\brak{\cos\theta-1\hspace{0.2cm} \sin\theta} r\begin{pmatrix}\cos\theta-1\\\sin\theta\end{pmatrix} \\
&= r^2 \brak{1+ \cos^2\theta + 2\cos\theta + \sin^2\theta}
\end{align}
Substituting the values of $\theta$ and $r$ , we get
\begin{align}
AC = 1.531
\label{eq: AC}
\end{align}

\item Expanding the L.H.S. of \eqref{eq:gen}
\begin{align}
&= r\brak{\cos\theta_1+1\hspace{0.2cm}\sin\theta_1} r\begin{pmatrix}
\cos\theta-1\\\sin\theta
\end{pmatrix} \\
&= r^2\brak{\brak{\cos\theta_1+1}\brak{\cos\theta-1}+\sin\theta\sin\theta_1} \\
&= r^2\brak{\cos\brak{\theta_1 - \theta}-\cos\theta_1+\cos\theta -1} \\
&= r^2\brak{\cos\beta-\cos\theta_1+\cos\theta -1}
\end{align}
Substituting value of $\beta$, $\theta_1$, $\theta$ and $r$, we get
\begin{align}
\brak{\vec{D}-\vec{B}}^T\brak{\vec{C} - \vec{A}} &= 1.864
\label{eq:LHS}
\end{align}
\item Substituting values from \eqref{eq: AC},\eqref{eq:BD} and \eqref{eq:LHS} in \eqref{eq:gen}, we get
\begin{align}
\cos\alpha &= 0.500 \\
\alpha &= 60\degree \\
\angle AEB &= 60\degree
\end{align}

Hence proved.
\end{enumerate}